backends/lean/Aeneas/Std/Core/Ops.lean
@@ -5,25 +5,25 @@ namespace Aeneas
 
 namespace Std
 
-open Result
+open RustM
 
 @[rust_trait "core::ops::index::Index"]
 structure core.ops.index.Index (Self Idx Output : Type) where
-  index : Self → Idx → Result Output
+  index : Self → Idx → RustM Output
 
 @[rust_trait "core::ops::index::IndexMut" (parentClauses := ["indexInst"])]
 structure core.ops.index.IndexMut (Self Idx Output : Type) where
   indexInst : Index Self Idx Output
-  index_mut : Self → Idx → Result (Output × (Output → Self))
+  index_mut : Self → Idx → RustM (Output × (Output → Self))
 
 @[rust_trait "core::ops::deref::Deref"]
 structure core.ops.deref.Deref (Self Target : Type) where
-  deref : Self → Result Target
+  deref : Self → RustM Target
 
 @[rust_trait "core::ops::deref::DerefMut" (parentClauses := ["derefInst"])]
 structure core.ops.deref.DerefMut (Self Target : Type) where
   derefInst : Deref Self Target
-  deref_mut : Self → Result (Target × (Target → Self))
+  deref_mut : Self → RustM (Target × (Target → Self))
 
 /-- Trait instance -/
 @[rust_trait_impl "core::ops::deref::Deref<Box<@T>, @T>" (keepParams := [true, false])]
@@ -42,36 +42,36 @@ def core.ops.deref.DerefMutBoxInst (T : Type) :
 
 @[rust_trait "core::ops::bit::BitAnd"]
 structure core.ops.bit.BitAnd (Self : Type) (Rhs : Type) (Self_Output : Type) where
-  bitand : Self → Rhs → Result Self_Output
+  bitand : Self → Rhs → RustM Self_Output
 
 @[rust_trait "core::ops::drop::Drop"]
 structure core.ops.drop.Drop (Self : Type) where
-  drop : Self → Result Self
+  drop : Self → RustM Self
 
 @[rust_fun "core::ops::drop::Drop::drop"]
 def core.ops.drop.Drop.drop.default {Self : Type}
-    (DropInst : core.ops.drop.Drop Self) : Self → Result Self :=
+    (DropInst : core.ops.drop.Drop Self) : Self → RustM Self :=
   fun s => DropInst.drop s
 
 @[rust_trait "core::ops::function::FnOnce"]
 structure core.ops.function.FnOnce (Self : Type u) (Args : Type v) (Output : Type w) where
-  call_once : Self → Args → Result Output
+  call_once : Self → Args → RustM Output
 
 @[rust_trait "core::ops::function::FnMut" (parentClauses := ["FnOnceInst"])]
 structure core.ops.function.FnMut (Self : Type u) (Args : Type v) (Output : Type w) where
   FnOnceInst : core.ops.function.FnOnce Self Args Output
-  call_mut : Self → Args → Result (Output × Self)
+  call_mut : Self → Args → RustM (Output × Self)
 
 @[rust_trait "core::ops::function::Fn" (parentClauses := ["FnMutInst"])]
 structure core.ops.function.Fn (Self : Type u) (Args : Type v) (Output : Type w) where
   FnMutInst : core.ops.function.FnMut Self Args Output
-  call : Self → Args → Result Output
+  call : Self → Args → RustM Output
 
-def BuiltinFnOnce (Inputs : Type u) (Outputs : Type v) : core.ops.function.FnOnce (Inputs → Result Outputs) Inputs Outputs := {
+def BuiltinFnOnce (Inputs : Type u) (Outputs : Type v) : core.ops.function.FnOnce (Inputs → RustM Outputs) Inputs Outputs := {
   call_once f x := f x
 }
 
-def BuiltinFnMut (Inputs : Type u) (Outputs : Type v) : core.ops.function.FnMut (Inputs → Result Outputs) Inputs Outputs := {
+def BuiltinFnMut (Inputs : Type u) (Outputs : Type v) : core.ops.function.FnMut (Inputs → RustM Outputs) Inputs Outputs := {
   FnOnceInst := BuiltinFnOnce Inputs Outputs
   call_mut f x :=
     match f x with
@@ -80,14 +80,14 @@ def BuiltinFnMut (Inputs : Type u) (Outputs : Type v) : core.ops.function.FnMut 
     | div => div
 }
 
-def BuiltinFn (Inputs : Type u) (Outputs : Type v) : core.ops.function.Fn (Inputs → Result Outputs) Inputs Outputs := {
+def BuiltinFn (Inputs : Type u) (Outputs : Type v) : core.ops.function.Fn (Inputs → RustM Outputs) Inputs Outputs := {
   FnMutInst := BuiltinFnMut Inputs Outputs
   call f x := f x
 }
 
 @[rust_trait "core::ops::try_trait::FromResidual"]
 structure core.ops.try_trait.FromResidual (Self : Type u) (R : Type v) where
-  from_residual : R → Result Self
+  from_residual : R → RustM Self
 
 @[rust_type "core::ops::control_flow::ControlFlow"]
 inductive core.ops.control_flow.ControlFlow (B : Type) (C : Type) where
@@ -97,8 +97,8 @@ inductive core.ops.control_flow.ControlFlow (B : Type) (C : Type) where
 @[rust_trait "core::ops::try_trait::Try" (parentClauses := ["FromResidualInst"])]
 structure core.ops.try_trait.Try (Self Output Residual : Type) where
   FromResidualInst : core.ops.try_trait.FromResidual Self Residual
-  from_output : Output → Result Self
-  branch : Self → Result (core.ops.control_flow.ControlFlow Residual Output)
+  from_output : Output → RustM Self
+  branch : Self → RustM (core.ops.control_flow.ControlFlow Residual Output)
 
 @[rust_trait "core::ops::try_trait::Residual" (parentClauses := ["TryInst"])]
 structure core.ops.try_trait.Residual (Self O TryType: Type) where
