backends/lean/Aeneas/Std/PrimitivesLemmas.lean
@@ -4,7 +4,7 @@ import Aeneas.Tactic.Conv.Bvify.Init
 
 namespace Aeneas.Std
 
-open Result WP
+open RustM WP
 
 @[step]
 theorem massert_spec (b : Prop) [Decidable b] :
