backends/lean/Aeneas/Std/Scalar/Misc.lean
@@ -4,7 +4,7 @@ import Mathlib.Data.BitVec
 
 namespace Aeneas.Std
 
-open Result Error Arith
+open RustM Error Arith
 
 /-- Important theorem to reason with `Int.bmod` in the proofs about `IScalar` -/
 theorem bmod_pow_numBits_eq_of_lt (ty : IScalarTy) (x : Int)
