backends/lean/Aeneas/Std/Scalar/SaturatingOps.lean
@@ -3,7 +3,7 @@ import Aeneas.Std.Scalar.Elab
 
 namespace Aeneas.Std
 
-open Result Error ScalarElab
+open RustM Error ScalarElab
 
 /-!
 # Saturating Operations
